olcoq/theories/Test.v
@@ -1,23 +1,99 @@
 Require Import OLPlugin.
-Require Import OL_Reflection_4_pointers.
+Require Import OL_Reflection_5_pointers.
+Require Import OL_Reflection_1_base.
 Require Import OL_Theory.
 
 Open Scope bool_scope.
+Require Import Btauto.
 
 
-Lemma foo : True. 
+Axiom False : forall (P:Prop), P.
 
-Proof.
-hello. 
-hello_ol.
-now auto.
-Qed.
+Ltac sorry := apply False.
 
-Example test8 : forall a b c: bool,  (a ∩ (negb a)) <= (a || (b && c)).
+
+Ltac ol_norm e := let e' := fresh "e" with Hol := fresh "Hol" in
+  olget e e'; assert (e = e') as Hol by (subst e'; (solveOLPointers BoolOL)); subst e'; try rewrite Hol; clear Hol.
+
+Ltac ol_norm_unsafe e := let e' := fresh "e" with Hol := fresh "Hol" in
+  olget e e'; assert (e = e') as Hol by sorry; subst e'; try rewrite Hol; clear Hol.
+
+Ltac ol_norm2 e := match e with 
+  | _ => 
+    lazymatch type of e with
+      | bool => ol_norm e
+      | _ => fail
+    end
+  | ?f ?arg => ol_norm2 f; ol_norm2 arg
+  | _ => idtac
+end.
+
+Ltac ol_norm2_unsafe e := match e with 
+  | _ => 
+    lazymatch type of e with
+      | bool => ol_norm_unsafe e
+      | _ => fail
+    end
+  | ?f ?arg => ol_norm2_unsafe f; ol_norm2_unsafe arg
+  | _ => idtac
+end.
+
+Ltac ol_norm3_unsafe := (lazymatch goal with
+  | [ |- ?e ] => ol_norm2_unsafe e
+end).
+
+
+
+Ltac ol_norm3 := (lazymatch goal with
+  | [ |- ?e ] => ol_norm2 e
+end).
+
+Tactic Notation "olnormalize" constr(e) := ol_norm2 e.
+Tactic Notation "olnormalize" := ol_norm3.
+
+
+Ltac destr_subbool e := 
+  lazymatch e with
+  | ?e1 <= ?e2 => first [destr_subbool e1 | destr_subbool e2]
+  | ?e1 = ?e2 => first [destr_subbool e1 | destr_subbool e2]
+  | true => fail
+  | false => fail
+  | (negb ?a) => destr_subbool a
+  | ?a && ?b => first [destr_subbool a | destr_subbool b]
+  | ?a || ?b => first [destr_subbool a | destr_subbool b]
+  | _ => destruct e
+  end.
+
+Ltac destr_subbool_goal := match goal with
+  | [ |- ?e ] => destr_subbool e
+end.
+
+Ltac oltauto := 
+  repeat (olnormalize; lazymatch goal with
+  | [ |- ?e1 = ?e1 ] => reflexivity
+  | [ |- ?e1 <= ?e1 ] => apply P1
+  | [ |- ?e ] => destr_subbool_goal
+  end).
+
+Example test9 : forall a b c: bool,  (a && (b || c) || (a && b) || (a && c)) = a && (b || c) && (a && b) || (a && c).
 Proof.
   intros.
-  olget ((a ∩ (negb a)) <= (a || (b && c))).
-  solveOLPointers BoolOL.
+(*olnormalize. *)
+  oltauto.
 Qed.
 
-Check test8.
+Example test10 : forall a b c: bool,  (a && (b || c) || (a && b) || (a && c)) = a && (b || c) && (a && b) || (a && c).
+Proof.
+  intros.
+  assert ((a && (b || c) || (a && b) || (a && c)) = a && (b || c) && (a && b) || (a && c)).
+  - destruct a; ol_norm3; reflexivity.
+  - destruct a; ol_norm3_unsafe; reflexivity.
+Qed.
+
+Example test8 : forall a b c: bool,  (a && (negb a)) <= (c || (b && negb b)).
+Proof.
+  intros.
+  olnormalize (a && (negb a)).
+  olnormalize.
+  solveOLPointers BoolOL.
+Qed.
